Full markup + bump Verso for new feature

Manual/ValidatingProofs.lean
@@ -7,11 +7,15 @@ import VersoManual
 
 import Manual.Meta
 
+import Verso.Code.External
+
 open Verso.Genre Manual
 open Verso.Genre.Manual.InlineLean
 
 set_option pp.rawOnError true
 set_option guard_msgs.diff true
+
+open Verso.Code.External (lit)
 
 open Lean (Syntax SourceInfo)
 
@@ -24,12 +28,12 @@ tag := "validating-proofs"
 This section discusses how to validate a proof expressed in Lean.
 
 Depending on the circumstances, additional steps may be recommended to rule out misleading proofs.
-In particular, it matters a lot whether one is dealing with an honest proof attempt, and needs protection against only benign mistakes, or a possibly-malicious proof attempt that actively tries to mislead.
+In particular, it matters a lot whether one is dealing with an {tech}[honest] proof attempt, and needs protection against only benign mistakes, or a possibly-{tech}[malicious] proof attempt that actively tries to mislead.
 
-In particular, we use “honest” when the goal is to create a valid proof.
+In particular, we use {deftech}_honest_ when the goal is to create a valid proof.
 This allows for mistakes and bugs in proofs and meta-code (tactics, attributes, commands, etc.), but not for code that clearly only serves to circumvent the system.
 
-In contrast, we use “malicious” to describe code to go out of its way to trick or mislead the user, exploit bugs or compromise the system.
+In contrast, we use {deftech}_malicious_ to describe code to go out of its way to trick or mislead the user, exploit bugs or compromise the system.
 This includes unreviewed AI-generated proofs and programs.
 
 Furthermore it is important to distinguish the question “does the theorem have a valid proof” from “what does the theorem statement mean”.
@@ -48,7 +52,7 @@ In regular everyday use of Lean, it suffices to check the blue double check mark
 While working interactively with Lean, once the theorem is proved, blue double check marks appear in the gutter to the left of the code.
 
 :::figure "A double blue check mark"
-![Double blue check marks appearing in the editor gutter](/static/screenshots/doublecheckmarks.png)
+![A theorem with double blue check marks appearing in the editor gutter](/static/screenshots/doublecheckmarks.png)
 :::
 
 ## Significance
@@ -57,7 +61,7 @@ The blue ticks indicate that the theorem statement has been successfully elabora
 
 ## Trust
 
-This check is meaningful if one believes the formal theorem statement corresponds to its intended informal meanings and trusts the authors of the imported libraries to be honest, that they performed this check, and that no unsound axioms have been declared and used.
+This check is meaningful if one believes the formal theorem statement corresponds to its intended informal meanings and trusts the authors of the imported libraries to be {tech}[honest], that they performed this check, and that no unsound axioms have been declared and used.
 
 ## Protection
 
@@ -65,8 +69,8 @@ This check is meaningful if one believes the formal theorem statement correspond
 This check protects against
 
 * Incomplete proof (missing goals, tactic error) *of the current theorem*
-* Explicit use of `sorry` *in the current theorem*
-* Honest bugs in meta-programs and tactics
+* Explicit use of {lean}`sorry` *in the current theorem*
+* {tech}[Honest] bugs in meta-programs and tactics
 * Proofs still being checked in the background
 :::
 
@@ -75,7 +79,7 @@ This check protects against
 In the Visual Studio Code extension settings, the symbol can be changed.
 Editors other than VS Code may have a different indication.
 
-Running `lake build +Module`, where `Module` refers to the file containing the theorem, and observing success without error messages or warnings provides the same guarantees.
+Running {lake}`build`{lit}` +Module`, where {lit}`Module` refers to the file containing the theorem, and observing success without error messages or warnings provides the same guarantees.
 
 # Printing Axioms
 %%%
@@ -87,20 +91,28 @@ Because both {lean}`sorry` and incomplete proofs are elaborated to axioms, their
 
 ## Instructions
 
-Write `#print axioms thmName` after the theorem declaration, with `thmName` replaced by the name of the theorem and check that it reports only the built-in axioms {name}`propext`, {name}`Classical.choice`, and {name}`Quot.sound`.
+:::keepEnv
+```lean -show
+inductive TheoremStatement : Prop where | intro
+theorem thmName : TheoremStatement := .intro
+```
+
+Write {leanCommand}`#print axioms thmName` after the theorem declaration, with {lean}`thmName` replaced by the name of the theorem and check that it reports only the built-in axioms {name}`propext`, {name}`Classical.choice`, and {name}`Quot.sound`.
+
+:::
 
 ## Significance
 
 This command prints the set of axioms used by the theorem and the theorems it depends on.
 The three axioms above are standard axioms of Lean's logic, and benign.
 
-* If {name}`sorryAx` is reported, then this theorem or one of its dependencies uses `sorry` or is otherwise incomplete.
-*  If {name}`Lean.trustCompiler` is reported, then native evaluation is used; see below for a discussion.
+* If {name}`sorryAx` is reported, then this theorem or one of its dependencies uses {lean}`sorry` or is otherwise incomplete.
+* If {name}`Lean.trustCompiler` is reported, then native evaluation is used; see below for a discussion.
 * Any other axiom means that a custom axiom was declared and used, and the theorem is only valid relative to the soundness of these axioms.
 
 ## Trust
 
-This check is meaningful if one believes the formal theorem statement corresponds to its intended informal meanings and one trusts the authors of the imported libraries to be honest.
+This check is meaningful if one believes the formal theorem statement corresponds to its intended informal meanings and one trusts the authors of the imported libraries to be {tech}[honest].
 
 ## Protection
 
@@ -108,16 +120,17 @@ This check is meaningful if one believes the formal theorem statement correspond
 (In addition to the list above)
 
 * Incomplete proofs
-* Explicit use of `sorry`
+* Explicit use of {lean}`sorry`
 * Custom axioms
 :::
 
 ## Comments
 
-At the time of writing, the `#print axioms` command does not work in a `module`.
-To work around this, create a non-module file, `import` your module, and use `#print axioms` there.
+At the time of writing, the {keywordOf Lean.Parser.Command.printAxioms}`#print axioms` command does not work in a {tech}[module].
+To work around this, create a non-module file, import your module, and use {keywordOf Lean.Parser.Command.printAxioms}`#print axioms` there.
 
-```leanModule
+```leanModule -show
+-- This module validates the claim in the preceding paragraph that #print axioms doesn't work here
 module
 /--
 error: cannot use `#print axioms` in a `module`; consider temporarily removing the `module` header or placing the command in a separate file
@@ -140,11 +153,11 @@ Build your project using {lake}`build`, run `lean4checker --fresh` on the module
 ## Significance
 
 The `lean4checker` tool reads the declarations and proofs as they are stored by `lean` during building (the {tech}[`.olean` files]), and replays them through the kernel.
-It trusts that the `.olean` files are structurally correct.
+It trusts that the {tech}[`.olean` files] are structurally correct.
 
 ## Trust
 
-This check is meaningful if one believes the formal theorem statement corresponds to its intended informal meanings and believes the authors of the imported libraries to not be very cunningly malicious, and to neither compromise the user’s system nor use Lean’s extensibility to change the interpretation of the theorem statement.
+This check is meaningful if one believes the formal theorem statement corresponds to its intended informal meanings and believes the authors of the imported libraries to not be very cunningly {tech}[malicious], and to neither compromise the user’s system nor use Lean’s extensibility to change the interpretation of the theorem statement.
 
 ## Protection
 
@@ -157,10 +170,10 @@ This check is meaningful if one believes the formal theorem statement correspond
 
 ## Comments
 
-Since `lean4checker` reads the `.olean` files without validating their format, this check is  prone to an attacker crafting invalid `.olean` files (e.g. invalid pointers, invalid data in strings).
+Since `lean4checker` reads the {tech}[`.olean` files] without validating their format, this check is  prone to an attacker crafting invalid `.olean` files (e.g. invalid pointers, invalid data in strings).
 
 Lean tactics and other meta-code can perform arbitrary actions when run.
-Importing libraries created by a determined malicious attacker and building them without further protection can compromise the user's system, after which no further meaningful checks are possible.
+Importing libraries created by a determined {tech}[malicious] attacker and building them without further protection can compromise the user's system, after which no further meaningful checks are possible.
 
 We recommend running `lean4checker` as part of CI for the additional protection against bugs in Lean's handling of declaration and as a deterrent against simple attacks.
 The [lean-action](https://github.com/leanprover/lean-action) Github Action provides this functionality by setting `lean4checker: true`.
@@ -172,7 +185,7 @@ Without the `--fresh` flag the tool can be instructed to only check some modules
 tag := "validating-comparator"
 %%%
 
-To protect against a seriously malicious proof compromising how Lean interprets a theorem statement or the user's system, additional steps are necessary.
+To protect against a seriously {tech}[malicious] proof compromising how Lean interprets a theorem statement or the user's system, additional steps are necessary.
 This should only be necessary for high risk scenarios (proof marketplaces, high-reward proof competitions).
 
 ## Instructions
@@ -181,20 +194,20 @@ In a trusted environment, write the theorem *statement* (the ”challenge”), a
 
 ## Significance
 
-Comparator will build the proof in a sandboxed environment, to protect against malicious code in the build step.
+Comparator will build the proof in a sandboxed environment, to protect against {tech}[malicious] code in the build step.
 The proof term is exported to a serialized format.
 Outside the sandbox and out of the reach of possibly malicious code, it validates the exported format, loads the proofs, replays them using Lean's kernel, and checks that the proved theorem statement matches the one in the challenge file.
 
 ## Trust
 
-This check is meaningful if the theorem statement in the trusted challenge file is correct and the sandbox used to build the possibly malicious code is safe.
+This check is meaningful if the theorem statement in the trusted challenge file is correct and the sandbox used to build the possibly-{tech}[malicious] code is safe.
 
 ## Protection
 
 :::listBullet "🛡️"
 (In addition to the list above)
 
-* Actively malicious proofs
+* Actively {tech}[malicious] proofs
 :::
 
 ## Comments
@@ -215,13 +228,13 @@ When following the gold standard of checking proofs using comparator, some assum
 # On `Lean.trustCompiler`
 
 Lean supports proofs by native evaluation.
-This is used by the `decide +native` tactic or internally by specific tactics ({tactic}`bv_decide` in particular) and produces proof terms that call compiled Lean code to do a calculation that is then trusted by the kernel.
+This is used by the {tactic}`decide`{keywordOf Lean.Parser.Tactic.decide}` +native` tactic or internally by specific tactics ({tactic}`bv_decide` in particular) and produces proof terms that call compiled Lean code to do a calculation that is then trusted by the kernel.
 
-Specific uses wrapped in honest tactics (e.g. {tactic}`bv_decide`) are generally trustworthy.
+Specific uses wrapped in {tech}[honest] tactics (e.g. {tactic}`bv_decide`) are generally trustworthy.
 The trusted code base is larger (it includes Lean's compilation toolchain and library annotations in the standard library), but still fixed and vetted.
 
-General use (`decide +native` or direct use of {name}`Lean.ofReduceBool`) can be used to create invalid proofs whenever the native evaluation of a term disagrees with the kernel's evaluation.
-In particular, all `implemented_by`/`extern` attributes in libraries become part of the trusted code base.
+General use ({tactic}`decide`{keywordOf Lean.Parser.Tactic.decide}` +native` or direct use of {name}`Lean.ofReduceBool`) can be used to create invalid proofs whenever the native evaluation of a term disagrees with the kernel's evaluation.
+In particular, all {attr}`implemented_by`/{attr}`extern` attributes in libraries become part of the trusted code base.
 
 All these uses show up as an axiom {name}`Lean.trustCompiler` in {keywordOf Lean.Parser.Command.printAxioms}`#print axioms`.
 External checkers (`lean4checker`, `comparator`) cannot check such proofs, as they do not have access to the Lean compiler.
